Update simproc for Map.find?
Also add ToString instances for PFlag and StateField.

Proofs/Sha512_block_armv8.lean
@@ -17,120 +17,95 @@ open BitVec
 -- Test 1: We have a 4 instruction program, and we attempt to simulate
 -- all of them.
 
--- def sha512_program_test_1 : Program :=
---   def_program
---     [(0x126538#64 , 0xcec08230#32),      --  sha512su0       v16.2d, v17.2d
---      (0x12653c#64 , 0x6e154287#32),      --  ext     v7.16b, v20.16b, v21.16b, #8
---      (0x126540#64 , 0xce6680a3#32),      --  sha512h q3, q5, v6.2d
---      (0x126544#64 , 0xce678af0#32)       --  sha512su1       v16.2d, v23.2d, v7.2d
---      ]
+def sha512_program_test_1 : Program :=
+  def_program
+    [(0x126538#64 , 0xcec08230#32),      --  sha512su0       v16.2d, v17.2d
+     (0x12653c#64 , 0x6e154287#32),      --  ext     v7.16b, v20.16b, v21.16b, #8
+     (0x126540#64 , 0xce6680a3#32),      --  sha512h q3, q5, v6.2d
+     (0x126544#64 , 0xce678af0#32)       --  sha512su1       v16.2d, v23.2d, v7.2d
+     ]
 
--- -- set_option profiler true in
--- -- set_option pp.deepTerms true in
--- theorem sha512_program_test_1_sym (s0 s_final : ArmState)
---   (h_s0_pc : read_pc s0 = 0x126538#64)
---   (h_s0_sp_aligned : CheckSPAlignment s0 = true)
---   (h_s0_program : s0.program = sha512_program_test_1)
---   (h_s0_ok : read_err s0 = StateError.None)
---   (h_run : s_final = run 4 s0) :
---   read_err s_final = StateError.None := by
---   -- Prelude
---   simp_all only [state_simp_rules, -h_run]
---   -- Symbolic simulation
---   sym_n 4 h_s0_program
---   -- simp (config := { contextual := true })
---   -- Final steps
---   unfold run at h_run
---   subst s_final s_4
---   simp_all only [state_simp_rules, minimal_theory, bitvec_rules]
---   done
+-- set_option profiler true in
+-- set_option pp.deepTerms true in
+theorem sha512_program_test_1_sym (s0 s_final : ArmState)
+  (h_s0_pc : read_pc s0 = 0x126538#64)
+  (h_s0_sp_aligned : CheckSPAlignment s0 = true)
+  (h_s0_program : s0.program = sha512_program_test_1)
+  (h_s0_ok : read_err s0 = StateError.None)
+  (h_run : s_final = run 4 s0) :
+  read_err s_final = StateError.None := by
+  -- Prelude
+  simp_all only [state_simp_rules, -h_run]
+  -- Symbolic simulation
+  sym_n 4 h_s0_program
+  -- Final steps
+  unfold run at h_run
+  subst s_final s4
+  simp_all only [state_simp_rules, minimal_theory, bitvec_rules]
+  done
 
--- ----------------------------------------------------------------------
+----------------------------------------------------------------------
 
--- -- Test 2: A 6 instruction program.
+-- Test 2: A 6 instruction program.
 
--- def sha512_program_test_2 : Program :=
---   def_program
---     [(0x126538#64 , 0xcec08230#32),      --  sha512su0       v16.2d, v17.2d
---      (0x12653c#64 , 0x6e154287#32),      --  ext     v7.16b, v20.16b, v21.16b, #8
---      (0x126540#64 , 0xce6680a3#32),      --  sha512h q3, q5, v6.2d
---      (0x126544#64 , 0xce678af0#32),      --  sha512su1       v16.2d, v23.2d, v7.2d
---      (0x126548#64 , 0x4ee38424#32),      --  add     v4.2d, v1.2d, v3.2d
---      (0x12654c#64 , 0xce608423#32)       --  sha512h2        q3, q1, v0
---      ]
+def sha512_program_test_2 : Program :=
+  def_program
+    [(0x126538#64 , 0xcec08230#32),      --  sha512su0       v16.2d, v17.2d
+     (0x12653c#64 , 0x6e154287#32),      --  ext     v7.16b, v20.16b, v21.16b, #8
+     (0x126540#64 , 0xce6680a3#32),      --  sha512h q3, q5, v6.2d
+     (0x126544#64 , 0xce678af0#32),      --  sha512su1       v16.2d, v23.2d, v7.2d
+     (0x126548#64 , 0x4ee38424#32),      --  add     v4.2d, v1.2d, v3.2d
+     (0x12654c#64 , 0xce608423#32)       --  sha512h2        q3, q1, v0
+     ]
 
--- -- set_option profiler true in
--- theorem sha512_program_test_2_sym (s0 s_final : ArmState)
---   (h_s0_pc : read_pc s0 = 0x126538#64)
---   (h_s0_program : s0.program = sha512_program_test_2)
---   (h_s0_ok : read_err s0 = StateError.None)
---   (h_run : s_final = run 6 s0) :
---   read_err s_final = StateError.None := by
---   -- Prelude
---   simp_all only [state_simp_rules, -h_run]
---   -- Symbolic simulation
---   sym_n 6 h_s0_program
---   -- Final steps
---   unfold run at h_run
---   subst s_final s_6
---   simp_all only [state_simp_rules, minimal_theory, bitvec_rules]
---   done
+-- set_option profiler true in
+theorem sha512_program_test_2_sym (s0 s_final : ArmState)
+  (h_s0_pc : read_pc s0 = 0x126538#64)
+  (h_s0_program : s0.program = sha512_program_test_2)
+  (h_s0_ok : read_err s0 = StateError.None)
+  (h_run : s_final = run 6 s0) :
+  read_err s_final = StateError.None := by
+  -- Prelude
+  simp_all only [state_simp_rules, -h_run]
+  -- Symbolic simulation
+  sym_n 6 h_s0_program
+  -- Final steps
+  unfold run at h_run
+  subst s_final s6
+  simp_all only [state_simp_rules, minimal_theory, bitvec_rules]
+  done
 
--- ----------------------------------------------------------------------
+----------------------------------------------------------------------
 
--- -- Test 3:
+-- Test 3:
 
--- def sha512_program_test_3 : Program :=
---   def_program
---    [(0x1264c0#64 , 0xa9bf7bfd#32),      --  stp     x29, x30, [sp, #-16]!
---     (0x1264c4#64 , 0x910003fd#32),      --  mov     x29, sp
---     (0x1264c8#64 , 0x4cdf2030#32),      --  ld1     {v16.16b-v19.16b}, [x1], #64
---     (0x1264cc#64 , 0x4cdf2034#32)       --  ld1     {v20.16b-v23.16b}, [x1], #64
---   ]
+def sha512_program_test_3 : Program :=
+  def_program
+   [(0x1264c0#64 , 0xa9bf7bfd#32),      --  stp     x29, x30, [sp, #-16]!
+    (0x1264c4#64 , 0x910003fd#32),      --  mov     x29, sp
+    (0x1264c8#64 , 0x4cdf2030#32),      --  ld1     {v16.16b-v19.16b}, [x1], #64
+    (0x1264cc#64 , 0x4cdf2034#32)       --  ld1     {v20.16b-v23.16b}, [x1], #64
+  ]
 
--- -- set_option profiler true in
--- -- set_option maxRecDepth 10000 in
--- set_option pp.deepTerms false in
--- set_option pp.deepTerms.threshold 10 in
--- theorem sha512_block_armv8_test_3_sym (s0 s_final : ArmState)
---   (h_s0_ok : read_err s0 = StateError.None)
---   (h_s0_sp_aligned : CheckSPAlignment s0 = true)
---   (h_s0_pc : read_pc s0 = 0x1264c0#64)
---   (h_s0_program : s0.program = sha512_program_test_3)
---   (h_run : s_final = run 4 s0) :
---   read_err s_final = StateError.None := by
---   -- Prelude
---   simp_all only [state_simp_rules, -h_run]
---   -- Symbolic simulation
---   sym_n 4 h_s0_program
---   -- Final steps
---   unfold run at h_run
---   subst s_final s_4
---   simp_all only [state_simp_rules, minimal_theory, bitvec_rules]
---   done
-
--- -- example: ofBool ((2#2).getLsb 1) = 1 := by
--- --   simp only [reduceGetLsb, ofBool_true, ofNat_eq_ofNat]
-
--- -- theorem test4 (s0 : ArmState) :
--- -- read_mem_bytes 16 (read_gpr 64 31#5 s0 + 18446744073709551600#64)
--- --  (w StateField.PC (1205444#64)
--- --     (w (StateField.GPR 31#5) (read_gpr 64 31#5 s0 + 18446744073709551600#64)
--- --       (write_mem_bytes (2 * ((8 <<< if (!0#1 == 1#1) = true then 2 + ((2#2).lsb 1).toNat else 2 + (2#2).toNat) / 8))
--- --         (read_gpr 64 31#5 s0 + 18446744073709551600#64)
--- --         (zeroExtend (8 <<< if (!0#1 == 1#1) = true then 2 + ((2#2).lsb 1).toNat else 2 + (2#2).toNat)
--- --             (r (StateField.GPR 30#5) s0) ++
--- --           zeroExtend (8 <<< if (!0#1 == 1#1) = true then 2 + ((2#2).lsb 1).toNat else 2 + (2#2).toNat)
--- --             (r (StateField.GPR 29#5) s0))
--- --         s0))) ==
--- --   (zeroExtend (8 <<< if (!0#1 == 1#1) = true then 2 + ((2#2).lsb 1).toNat else 2 + (2#2).toNat)
--- --             (r (StateField.GPR 30#5) s0) ++
--- --           zeroExtend (8 <<< if (!0#1 == 1#1) = true then 2 + ((2#2).lsb 1).toNat else 2 + (2#2).toNat)
--- --             (r (StateField.GPR 29#5) s0)) := by
--- --           simp (config := {decide := true}) [state_simp_rules, minimal_theory, bitvec_rules, lsb, reduceGetLsb, ofBool_true, ofNat_eq_ofNat]
--- --           apply read_mem_bytes_of_write_mem_bytes_same
--- --           simp only [Nat.reducePow, Nat.reduceLeDiff]
--- --           done
+-- set_option profiler true in
+set_option pp.deepTerms false in
+set_option pp.deepTerms.threshold 10 in
+theorem sha512_block_armv8_test_3_sym (s0 s_final : ArmState)
+  (h_s0_ok : read_err s0 = StateError.None)
+  (h_s0_sp_aligned : CheckSPAlignment s0 = true)
+  (h_s0_pc : read_pc s0 = 0x1264c0#64)
+  (h_s0_program : s0.program = sha512_program_test_3)
+  (h_run : s_final = run 4 s0) :
+  read_err s_final = StateError.None := by
+  -- Prelude
+  simp_all only [state_simp_rules, -h_run]
+  -- Symbolic simulation
+  sym_n 4 h_s0_program
+  -- Final steps
+  unfold run at h_run
+  subst s_final s4
+  simp_all only [state_simp_rules, minimal_theory, bitvec_rules]
+  done
 
 ----------------------------------------------------------------------
 
@@ -139,6 +114,7 @@ open BitVec
 -- we'd like to verify).
 
 -- set_option profiler true in
+-- set_option profiler.threshold 10 in
 theorem sha512_block_armv8_test_4_sym (s0 s_final : ArmState)
   (h_s0_ok : read_err s0 = StateError.None)
   (h_s0_sp_aligned : CheckSPAlignment s0 = true)
@@ -149,25 +125,57 @@ theorem sha512_block_armv8_test_4_sym (s0 s_final : ArmState)
   -- Prelude
   simp_all only [state_simp_rules, -h_run]
   -- Symbolic simulation
+  -- sym_n 5 h_s0_program
   -- sym_i_n 0 1 h_s0_program
+  -- init_next_step h_run
+  -- rename_i s1 h_step_1 h_run
+  -- -- fetch_and_decode_inst h_step_1 h_s0_program
+  -- simp only [*, stepi, state_simp_rules, minimal_theory, bitvec_rules] at h_step_1
+  -- rw [fetch_inst_from_program] at h_step_1
+  -- simp only [h_s0_program] at h_step_1
+  -- conv at h_step_1 =>
+  --   pattern Map.find? _ _
+  --   tactic => set_option maxRecDepth 3000 in
+  --             simp (config := {ground := true}) only [reduceMapFind?]
+  -- (try dsimp only at h_step_1)
+  -- conv at h_step_1 =>
+  --   pattern decode_raw_inst _
+  --   tactic =>
+  --     simp (config := {ground := true}) only
+  -- (try dsimp only at h_step_1)
+  -- simp (config := {decide := true}) only
+  --   [exec_inst, state_simp_rules, minimal_theory]
+  --   at h_step_1
+  sym_i_n 0 1 h_s0_program
   init_next_step h_run
-  rename_i s1 h_step_1 h_run
-  -- fetch_and_decode_inst h_step_1 h_s0_program
-  simp only [*, stepi, state_simp_rules, minimal_theory, bitvec_rules] at h_step_1
-  rw [fetch_inst_from_program] at h_step_1
-  simp only [h_s0_program] at h_step_1
-  conv at h_step_1 =>
+  rename_i s2 h_step_2 h_run
+  -- fetch_and_decode_inst h_step_2 h_s0_program
+  simp only [stepi, state_simp_rules, minimal_theory, bitvec_rules] at h_step_2
+  rw [fetch_inst_from_program] at h_step_2
+  have h_s1_program : s1.program = s0.program := by
+    simp_all only [state_simp_rules, minimal_theory, bitvec_rules]
+  have h_s1_err : r StateField.ERR s1 = StateError.None := by
+    simp_all only [state_simp_rules, minimal_theory, bitvec_rules]
+  have h_s1_pc : r StateField.PC s1 = (1205444#64) := by
+    simp_all only [state_simp_rules, minimal_theory, bitvec_rules]
+  simp only [h_s0_program, h_s1_program, h_s1_err, h_s1_pc] at h_step_2
+  conv at h_step_2 =>
     pattern Map.find? _ _
-    tactic => set_option maxRecDepth 1200 in
-              -- simp (config := {ground := true}) only
-              simp only [sha512_program_map, def_program, reduceMapFind?]
-  dsimp only at h_step_1
-  conv at h_step_1 =>
+    tactic => set_option maxRecDepth 3000 in
+              simp only [reduceMapFind?]
+  (try dsimp only at h_step_2)
+  conv at h_step_2 =>
     pattern decode_raw_inst _
-    tactic => simp (config := {ground := true}) only
-  dsimp only at h_step_1
-  --
-  exec_inst h_step_1
+    tactic =>
+      simp (config := {ground := true}) only
+  (try dsimp only at h_step_2)
+  (try clear h_s1_program h_s1_err)
+  -- exec_inst h_step_2
+  have h_s1_gpr31 : r (StateField.GPR 31#5) s1 = (r (StateField.GPR 31#5) s0 + 18446744073709551600#64) := by
+    simp_all only [stepi, state_simp_rules, minimal_theory, bitvec_rules]
+  simp (config := { decide := true }) only [*, -h_step_1, exec_inst, state_simp_rules, minimal_theory, bitvec_rules] at h_step_2
+  (try (repeat simp (config := {ground := true}) only [↓reduceIte, state_simp_rules, minimal_theory, bitvec_rules] at h_step_2))
+
   sorry
 
 ----------------------------------------------------------------------
